Add CPUID test for the RDSEED feature

experimental/cpuid/Test.Hacl.Hardware.Intel.CPUID.fst
@@ -10,18 +10,18 @@ open Hacl.Hardware.Intel.CPUID
 
 
 (* Detect if the processor is an Intel CPU *)
-val detect_intel_cpu: unit 
+val detect_intel_cpu: unit
   -> Stack bool
           (requires (fun h -> True))
           (ensures  (fun h0 _ h1 -> h0 == h1))
 let detect_intel_cpu () = if (_is_intel_cpu() = 1ul) then true else false
 
 
-(* Detect if the processor has support for the DRNG features *)
+(* Detect if the processor has support for the RDRAND DRNG feature *)
 val detect_intel_feature_rdrand: unit
   -> Stack bool (requires (fun h0 -> True))
                (ensures  (fun h0 _ h1 -> modifies_0 h0 h1))
-               
+
 let detect_intel_feature_rdrand () =
   push_frame();
   let features = { eax = 0ul; ebx = 0ul; ecx = 0ul; edx = 0ul; } in
@@ -39,9 +39,31 @@ let detect_intel_feature_rdrand () =
   r
 
 
+(* Detect if the processor has support for the RDSEED DRNG feature *)
+val detect_intel_feature_rdseed: unit
+  -> Stack bool (requires (fun h0 -> True))
+               (ensures  (fun h0 _ h1 -> modifies_0 h0 h1))
+
+let detect_intel_feature_rdseed () =
+  push_frame();
+  let features = { eax = 0ul; ebx = 0ul; ecx = 0ul; edx = 0ul; } in
+  let rfeatures = Buffer.create features 1ul in
+  let r =
+    match detect_intel_cpu () with
+    | false -> false
+    | true ->
+      (* Retrieve the cpuid information from the CPU *)
+      cpuid rfeatures 7ul 0ul;
+      (* Check the bit for the RDSEED feature *)
+      if ((let a = rfeatures.(0ul) in a.ebx &^ 0x40000ul) =^ 0x40000ul) then true else false
+  in
+  pop_frame();
+  r
+
+
 (* Entry point *)
 let main () =
-  
+
   (* Detect if the machine is an Intel CPU *)
   (match detect_intel_cpu () with
   | true  -> C.print_string (C.string_of_literal " * CPU Information: Intel processor detected on your machine.\n")
@@ -50,6 +72,11 @@ let main () =
   (* Detect if the machine supports the RDRAND feature *)
   (match detect_intel_feature_rdrand () with
   | true -> C.print_string (C.string_of_literal " *         Feature: Digital Random Number Generator (RDRAND)\n")
+  | false -> ());
+
+  (* Detect if the machine supports the RDSEED feature *)
+  (match detect_intel_feature_rdseed () with
+  | true -> C.print_string (C.string_of_literal " *         Feature: Digital Random Number Generator (RDSEED)\n")
   | false -> ());
 
   C.exit_success
